some stylistic changes

examples/algorithms/IntervalIntersect.fst
@@ -4,6 +4,7 @@ open FStar.All
 open FStar.List.Tot
 open FStar.IO
 open FStar.Printf
+open FStar.Math.Lib
 
 ///[from] is inclusive, [to] is not inclusive
 type interval = | I: from:int -> to:int{from<to} -> interval
@@ -11,35 +12,34 @@ type interval = | I: from:int -> to:int{from<to} -> interval
 let rec goodLIs (is:list interval) (lb:int) =
   match is with
   | [] -> true
-  | (I f t :: is) -> lb <= f && f < t && goodLIs is t
+  | I f t :: is -> lb <= f
+                 //&& f < t  NS: unnecessary
+                 && goodLIs is t
 
-let good is = 
+let good is =
   match is with
   | [] -> true
-  | (I f t :: _) -> goodLIs is f 
+  | I f t :: _ -> goodLIs is f
 
-let intervals = is:(list interval){good is}
+let intervals = is:list interval{good is}
 
-let needs_reorder (is1:intervals) (is2:intervals): nat =
+let needs_reorder (is1 is2:intervals) : nat =
   match is1, is2 with
-  | (I f1 t1 :: _), (I f2 t2 :: _) -> if (t1 < t2) then 1 else 0
+  | I f1 t1 :: _, I f2 t2 :: _ -> if t1 < t2 then 1 else 0
   | _, _ -> 0
 
-let max = Math.Lib.max
-let min = Math.Lib.min
-
-val go: is1:intervals -> is2:intervals -> Pure (ris:intervals) 
-  (requires True)
-  (ensures (fun ris -> True
-    /\ ( Cons? ris /\ Cons? is1 /\ Cons? is2 ==> 
-        (hd ris).from >= max ((hd is1).from) ((hd is2).from)  )
-    /\ ( Nil? is1 \/ Nil? is2 ==> Nil? ris )))
-  (decreases %[List.length is1 + List.length is2; needs_reorder is1 is2])
-let rec go is1 is2 =
+let rec go (is1 is2:intervals)
+  : Pure intervals
+         (requires True)
+         (ensures (fun ris ->
+            ( Cons? ris /\ Cons? is1 /\ Cons? is2 ==>
+             (hd ris).from >= max (hd is1).from (hd is2).from  )
+         /\ ( Nil? is1 \/ Nil? is2 ==> Nil? ris )))
+         (decreases %[List.length is1 + List.length is2; needs_reorder is1 is2]) =
   match is1, is2 with
   | _, [] -> []
   | [], _ -> []
-  | (i1::is1), (i2::is2) ->
+  | i1::is1, i2::is2 ->
     begin
       let f' = max (i1.from) (i2.from) in
       // reorder for symmetry
@@ -53,23 +53,19 @@ let rec go is1 is2 =
         go (I (i2.to) (i1.to) :: is1) is2
     end
 
-val intersect: is1:intervals -> is2:intervals -> ris:intervals
-let intersect is1 is2 =
-  go is1 is2
+let intersect (is1 is2:intervals) = go is1 is2
 
 let rec print_intervals is: ML unit =
   match is with
-  | [] -> (print_string ".")
+  | [] -> stdout <| "."
   | (i::is) ->
-    begin
-      print_string (sprintf "[%d, %d] " i.from i.to);
-      print_intervals is
-    end
+    stdout <| sprintf "[%d, %d] " i.from i.to;
+    print_intervals is
 
 let main = print_intervals (intersect [I 3 10; I 11 15] [I 1 4; I 10 14])
 
 let range (f:int) (t:int): Set.set int =
-  Set.intension (fun z -> (f <= z) && (z < t))
+  Set.intension (fun z -> f <= z && z < t)
 
 let semI (i : interval) : Set.set int =
   range i.from i.to
@@ -79,31 +75,30 @@ let rec sem (is : intervals) : Set.set int =
   | [] -> Set.empty #int
   | (i :: is) -> Set.union (semI i) (sem is)
 
-val lemma_disjoint_intro: #a:eqtype -> s1:Set.set a -> s2:Set.set a -> Lemma
-  (requires Set.equal (Set.intersect s1 s2) Set.empty)
-  (ensures Set.disjoint s1 s2)
-  [SMTPat (Set.disjoint s1 s2)]
-let lemma_disjoint_intro #a s1 s2 = ()
+let lemma_disjoint_intro (#a:eqtype) (s1 s2:Set.set a)
+  : Lemma
+    (requires Set.equal (Set.intersect s1 s2) Set.empty)
+    (ensures Set.disjoint s1 s2)
+    [SMTPat (Set.disjoint s1 s2)]
+ = ()
 
-val lemma_intersection_range_range: f1:int -> t1:int -> f2:int -> t2:int -> Lemma
-  (requires True)
-  (ensures (Set.intersect (range f1 t1) (range f2 t2)) == (range (max f1 f2) (min t1 t2)))
-let lemma_intersection_range_range f1 t1 f2 t2 =
-  Set.lemma_equal_elim (Set.intersect (range f1 t1) (range f2 t2)) (range (max f1 f2) (min t1 t2));
-  ()
+let lemma_intersection_range_range (f1 t1 f2 t2:int)
+  : Lemma
+    (ensures (Set.intersect (range f1 t1) (range f2 t2) == range (max f1 f2) (min t1 t2)))
+  = Set.lemma_equal_elim (Set.intersect (range f1 t1) (range f2 t2))
+                         (range (max f1 f2) (min t1 t2))
 
-val lemma_intersection_range_range_empty: f1:int -> t1:int -> f2:int -> t2:int -> Lemma
-  (requires (t1 <= f2) \/ (t2 <= f1))
-  (ensures Set.intersect (range f1 t1) (range f2 t2) == Set.empty)
-let lemma_intersection_range_range_empty f1 t1 f2 t2 =
-  Set.lemma_equal_elim ( Set.intersect (range f1 t1) (range f2 t2) ) Set.empty;
-  ()
+let lemma_intersection_range_range_empty (f1 t1 f2 t2:int)
+  : Lemma
+    (requires (t1 <= f2) \/ (t2 <= f1))
+    (ensures Set.intersect (range f1 t1) (range f2 t2) == Set.empty)
+  = Set.lemma_equal_elim ( Set.intersect (range f1 t1) (range f2 t2) ) Set.empty
 
 val lemma_intersection_range_semLIs_empty: f:int -> t:int -> is:intervals -> lb:int -> Lemma
   (requires goodLIs is lb /\ t <= lb)
   (ensures Set.intersect (range f t) (sem is) == Set.empty)
 
-let rec lemma_intersection_range_semLIs_empty f t is lb = 
+let rec lemma_intersection_range_semLIs_empty f t is lb =
   if (Cons? is) then
     begin
       lemma_intersection_range_semLIs_empty f t (tl is) (hd is).to
@@ -115,7 +110,7 @@ let rec lemma_intersection_range_semLIs_empty f t is lb =
 val lemma_intervals_disjoint: is:intervals{Cons? is} -> Lemma
   (requires True)
   (ensures (Set.disjoint (semI (hd is)) (sem (tl is))))
-let lemma_intervals_disjoint is = 
+let lemma_intervals_disjoint is =
   if (Cons? (tl is)) then
     begin
       let h::t = is in
@@ -144,25 +139,25 @@ val lemma_intersection_spec: is1:intervals -> is2 : intervals -> Lemma
   (ensures (Set.equal ( sem (intersect is1 is2) ) (Set.intersect (sem is1) (sem is2))))
   (decreases %[List.length is1 + List.length is2; needs_reorder is1 is2])
 
-let rec lemma_intersection_spec is1 is2 = 
+let rec lemma_intersection_spec is1 is2 =
   match is1, is2 with
   | [], [] -> ()
-  | _, [] -> () 
+  | _, [] -> ()
   | [], _ -> ()
-  | (i1::is1), (i2::is2) -> 
-    begin 
+  | (i1::is1), (i2::is2) ->
+    begin
        let f_max = max (i1.from) (i2.from) in
        let f_min = min (i1.from) (i2.from) in
        // reorder for symmetry
        if i1.to < i2.to then lemma_intersection_spec (i2::is2) (i1::is1)
        // disjoint i2.from, i2.to, i1.from, i1.to
-       else if i1.from >= i2.to then ( 
+       else if i1.from >= i2.to then (
          lemma_intersection_spec (i1::is1) is2;
          assert (Set.disjoint (semI i1) (semI i2));
          lemma_disjoint_prefix (i1::is1) (i2::is2);
-         () 
+         ()
        )
-       // subset f_min, f_max, i1.to=i1.to, 
+       // subset f_min, f_max, i1.to=i1.to,
        else if i1.to = i2.to then (
          assert (Set.equal (Set.intersect (semI i1) (semI i2)) (semI (I f_max i1.to)));
          lemma_intervals_disjoint (i2::is1);
@@ -171,11 +166,11 @@ let rec lemma_intersection_spec is1 is2 =
          ()
        )
        // overlapping
-       else  ( 
-         ignore (I f_max (i2.to)); 
+       else  (
+         ignore (I f_max (i2.to));
          assert (Set.equal (Set.intersect (semI i1) (semI i2)) (semI (I f_max i2.to)));
          lemma_intervals_disjoint (i2::is1);
-         lemma_intersection_spec (I (i2.to) (i1.to) :: is1) is2; 
-         admit() 
+         lemma_intersection_spec (I (i2.to) (i1.to) :: is1) is2;
+         admit()
        )
     end
